$$
\begin{array}{l}
\mathlarger{\boxed{Γ ⊢ A \haskind χ}}\ \text{Under context $Γ$, type $A$ has kind $χ$}
\end{array}
$$

\begin{mathpar}

\inferrule*[right=KindVar]
{ (α : χ) ∈ Γ }
{ Γ ⊢ α \haskind χ }

\and
\inferrule*[right=KindFree]
{ (\Type : χ) ∈ Φ }
{ Γ ⊢ \Type \haskind χ }

\and
\inferrule*[right=Kind$→$]
{ Γ ⊢ A \haskind ⋆ \\ Γ ⊢ B \haskind ⋆ }
{ Γ ⊢ A → B \haskind ⋆ }

\and
\inferrule*[right=KindTuple]
{ Γ ⊢ A_1 \haskind ⋆ \\ \dots \\ Γ ⊢ A_n \haskind ⋆ }
{ Γ ⊢ ⟨A_1, \dots, A_n ⟩ \haskind ⋆ }

\and
\inferrule*[right=Kind$∀$]
{ Γ, α : χ ⊢ A \haskind ⋆ }
{ Γ ⊢ ∀α : χ.\, A \haskind ⋆ }

\and
\inferrule*[right=KindApp]
{ Γ ⊢ F \haskind (χ_1 → χ_2) \\ Γ ⊢ B \haskind χ_1 }
{ Γ ⊢ F\, B \haskind χ_2 }

\and
\inferrule*[right=KindFix]
{ Γ ⊢ F \haskind (⋆ → ⋆) }
{ Γ ⊢ \sym{Fix}\, F \haskind ⋆ }

\and
\inferrule*[right=Kind$\latkap$]
{ Γ ⊢ κ \haskind \clockk \\ Γ ⊢ A \haskind ⋆ }
{ Γ ⊢ \latkap{A} \haskind ⋆ }

\inferrule*[right=KindEVar]
{ \ahat : χ ∈ Γ }
{ Γ ⊢ \ahat \haskind χ }

\and
\inferrule*[right=KindEVarSolved]
{ \ahat : χ = τ ∈ Γ }
{ Γ ⊢ \ahat \haskind χ }

\end{mathpar}
