$$
\def\arraystretch{1.2}
\begin{array}{l}
\mathlarger{\boxed{Γ ⊢ e \checks A ⊣ Δ}}\ \text{Under input context $Γ$, $e$ checks against type $A$,
            with output context $Δ$} \\
\mathlarger{\boxed{Γ ⊢ e \synths A ⊣ Δ}}\ \text{Under input context $Γ$, $e$ synthesizes type $A$,
            with output context $Δ$}  \\
\mathlarger{\boxed{Γ ⊢ A \bull e \appsynths C ⊣ Δ}}\
  \begin{array}[t]{l}
  \text{Under input context $Γ$, applying a function of type $A$ to $e$}\\
  \text{synthesizes type $C$, with output context $Δ$}
  \end{array} \\
\end{array}
$$
\begin{mathpar}

\inferrule*[right=Var]
{(x : A) ∈ Γ}
{Γ ⊢ x \synths A ⊣ Γ}

\inferrule*[right=\Decl Constr$\synths$]
{ (\Constr : A) ∈ Φ }
{ Γ ⊢ \Constr \synths A ⊢ Γ }

\and
\inferrule*[right=Anno]
{Γ ⊢ A \\ Γ ⊢ e \checks A ⊣ Δ}
{Γ ⊢ (e : A) \synths A ⊣ Δ}

\and
\inferrule*[right=$∀$I]
{ Γ, α \hask χ ⊢ e \checks A ⊣ Δ,α,Θ }
{ Γ ⊢ e \checks ∀α \hask χ.\ A ⊣ Δ }

\and
\inferrule*[right=$∀$App,leftskip=3em]
{ Γ,\ahat \hask χ ⊢ [\ahat/α]A \bull e \appsynths C ⊣ Δ}
{ Γ ⊢ ∀α \hask χ.\ A \bull e \appsynths C ⊣ Δ }

\and
\inferrule*[right=$→$I,leftskip=3em]
{ Γ,x:A ⊢ e \checks B ⊣ Δ, x:A, Θ}
{ Γ ⊢ λx.\, e \checks A → B ⊣ Δ }

\and
\inferrule*[right=Sub]
{Γ ⊢ e \synths A ⊣ Θ \\ Θ ⊢ [Θ]A \subt [Θ]B ⊣ Δ}
{Γ ⊢ e \checks B ⊣ Δ}

\and
\inferrule*[right=$→$I$\synths$]
{ Γ,\ahat,\bhat, x:\ahat ⊢ e \checks \bhat ⊣ Δ,x:\ahat,Θ }
{ Γ ⊢ λx.\, e \synths \ahat → \bhat ⊣ Δ }

\and
\inferrule*[right=$→$E]
{ Γ ⊢ e₁ \synths A ⊣ Θ \\ Θ ⊢ [Θ]A \bull e_2 \appsynths C ⊣ Δ }
{ Γ ⊢ e₁\, e₂ \synths C ⊣ Δ }

\and
\inferrule*[right=$\ahat$App]
{ Γ[\ahatk[⋆][2], \ahatk[⋆][1], \ahatk[⋆] = \ahat_1 → \ahat_2] ⊢ e \checks \ahat_1 ⊣ Δ }
{ Γ[\ahatk[⋆]] ⊢ \ahat \bull e \appsynths \ahat_2 ⊣ Δ }

\and
\inferrule*[right=$\latkap\ahat$App]
{ Γ[\ahatk[χ][2], \ahatk[\clockk][1], \ahatk[⋆] = \latkap[\ahat_1] \ahat_2] ⊢ x \checks \ahat_1 ⊣ Δ }
{ Γ[\ahatk[⋆]] ⊢ \ahat \bull [x] \appsynths \ahat_2 ⊣ Δ }

\and
\inferrule*[right=$→$App]
{ Γ ⊢ e \checks A ⊣ Δ }
{ Γ ⊢ A → C \bull e \appsynths C ⊣ Δ }

\and
\inferrule*[right=TupleI$\synths$]
{ Γ ⊢ e_1 \synths A_1 ⊣ Δ_1 \ \dots \ Δ_{n-1} ⊢ e_n \synths A_n ⊣ Δ_n }
{ Γ ⊢ ⟨e_1, \dots, e_n⟩ \synths ⟨A_1, \dots, A_n) ⊣ Δ_n }

\and
\inferrule*[right=TupleI]
{ Γ ⊢ e_1 \checks A_1 ⊣ Δ_1 \ \dots \ Δ_{n-1} ⊢ e_n \checks A_n ⊣ Δ_n }
{ Γ ⊢ ⟨e_1, \dots, e_n⟩ \checks ⟨A_1, \dots, A_n) ⊣ Δ_n }

\and
\inferrule*[right=$\latkap$I$\synths$]
{ Γ ⊢ κ \haskind \clockk \\ Γ,x :_λ κ ⊢ e \synths A ⊣ Δ }
{ Γ ⊢ γ(x : κ).\, e \synths \latkap A ⊣ Δ }

\and
\inferrule*[right=TApp]
{ Γ ⊢ e \synths ∀(α : χ).\ B ⊣ Δ \\ Δ ⊢ A \haskind χ }
{ Γ ⊢ e\, \{A\} \synths [A/α]B ⊣ Δ }

% \and
% \inferrule*[right=Fold$\synths$]
% {  }
% { Γ ⊢ \sym{fold} \synths ∀(α : ⋆ → ⋆).\ α\, (\Rec\, α) → \Rec\, α ⊣ Γ }

\and
\inferrule*[right=$\latkap$App]
{ Γ ⊢ κ \haskind \clockk \\ Γ ⊢ x \checks κ ⊣ Δ }
{ Γ ⊢ (\latkap\, A) \bull [x] \appsynths A ⊣ Δ }

% \and
% \inferrule*[right=Unfold$\synths$]
% {  }
% { Γ ⊢ \sym{unfold} \synths ∀(α : ⋆ → ⋆).\ \Rec\, α → α\, (\Rec\, α) ⊣ Γ }

\and
\inferrule*[right=$\latkap$App$\tickc$]
{ Γ ⊢ κ \haskind \clockk \\ \stable_κ(Γ) }
{ Γ ⊢ (\latkap\, A) \bull [\tickc] \appsynths A ⊣ Γ }

% \and
% \inferrule*[right=Fix]
% { }
% { Γ ⊢ \sym{fix} \synths ∀(κ : \clockk), α.\ (\latkap α → α) → α ⊣ Γ }

% \and
% \inferrule*[right=Fmap,leftskip=4em]
% { Functor(F) ∈ Φ }
% { Γ ⊢ \sym{fmap}_F \synths ∀α, β.\ (α → β) → F\, α → F\, β ⊣ Γ }

% \and
% \inferrule*[right=PrimRec]
% { Functor(F) ∈ Φ }
% { Γ ⊢ \sym{primRec}_F \synths ∀α.\ F\, ⟨\Rec\, F, α⟩ → \Rec\, F → α ⊣ Γ }

\and
\inferrule*[right=Case]
{ Γ ⊢ e \synths A \\ (A',Θ) = intros(A,Γ) \\ Θ ⊢ \checkbranch{ρ_1}{[Θ]A'}{e_1}{[Θ]B} ⊢ Δ_1
  \ \dots \
  Δ_{n-1} ⊢ \checkbranch{ρ_n}{[Δ_{n-1}]A'}{e_n}{B} ⊣ Δ_n
}
{ Γ ⊢ \case\ e\ \sym{of}\ (\branch{1}, \dots, \branch{n}) \checks B ⊣ Δ_n }
\end{mathpar}
